template-coq/src/reification.ml
@@ -48,6 +48,7 @@ sig
   type quoted_constant_body
   type quoted_global_decl
   type quoted_global_declarations
+  type quoted_retroknowledge
   type quoted_global_env
   type quoted_program  (* the return type of quote_recursively *)
 
